proof: reorg

theories/Operational/Security.v
@@ -4,228 +4,23 @@ Require Import List.
 Require Import Logic.Eqdep_dec Logic.EqdepFacts.
 Require Import Unicode.Utf8.
 
-Require Import config.
-Require Import data_model.
-Require Import expression.
-Require Import lattice.
-Require Import relation.
-Require Import semantics.
-Require Import trace.
-Require Import types.
-Require Import util.
-Require Import termination.
+Require Import Base.Config.
+Require Import Base.Lattice.
+Require Import Base.Ordering.
+Require Import Base.Trace.
+Require Import Base.Types.
+Require Import Base.Util.
+
+Require Import Data.DataModel.
+Require Import Data.Relation.
+
+Require Import Experimental.Udf.
+Require Import Experimental.Termination.
+
+Require Import Operational.Expression.
+Require Import Operational.Semantics.
 
 Section SecurityMain.
-
-(*
- * Checks whether a policy p1 can be downgraded to p2 using op.
- *)
-Definition valid_prov (τ: prov_type) (p1 p2: Policy.policy): Prop :=
-  (*
-   * First of all we must ensure that the level of policies are lowered, which would
-   * otherwise make no sense at all.
-   *)
-  p2 ⪯ p1 ∧
-  (*
-   * Next we check if `p1` can be "lowered". This is ensured by `p1` ⪯ `∘ op`
-   *)
-    match τ with
-      (*
-      * Adding `p ⪯ ∘ op` should be enough for the condition as this is equivalent to
-      * `(first label p) ⊑ op`, the proof of which is trivial and intuitive.
-      *)
-      | prov_trans_unary op => p2 ⪯ (∘ (Policy.policy_transform ((UnaryTransOp op) :: nil)))
-      | prov_trans_binary bt op v => p2 ⪯ (∘ (Policy.policy_transform ((BinaryTransOp bt op v) :: nil)))
-      | prov_agg op => p2 ⪯ (∘ (Policy.policy_agg (op :: nil)))
-      | prov_noise op => p2 ⪯ (∘ (Policy.policy_noise op))
-      | _ => True
-    end
-.
-
-(*
- * For a cell to be released (i.e., it can be shared freely), it must be the case that all policies are satisfied.
- * Fortunately, we have `policy_clean`. This means that we can just check whether the policy is clean.
- *)
-Definition can_release p: Prop := p = ∎.
-
-(* TODO: Define this. *)
-Definition budget_bounded (β: budget): Prop := True.
-
-Notation "p1 '=[' p ']=>' p2" := (valid_prov p p1 p2)
-  (at level 10, p at next level, p2 at next level).
-
-(* 
- *                      ----< tr1
- *                     /
- * trace: join / agg --< lbl  -----< tr2
- *                     \
- *                      ----< ...
- *)
-Inductive branch_ok: Policy.policy → list trace_ty → Prop :=
-  | BranchEmptyOk: ∀ lbl, branch_ok lbl nil
-  | BranchConsOk: ∀ lbl lbl1 tr hd tl,
-      tr = hd :: tl →
-      lbl1 = extract_policy hd →
-      lbl1 ⪯ lbl →
-      branch_ok lbl tl →
-      branch_ok lbl tr
-.
-
-(*
- * Checks against for each element, can it be released via the current label?
- *)
-Inductive valid_transition: prov_type → Policy.policy → trace_ty → Prop :=
-  (* tr: old (higher) *)
-  (* lbl: new (lower) *)
-  | ValidTransition: ∀ prov lbl lbl' tr,
-      lbl' = extract_policy tr →
-      lbl' =[ prov ]=> lbl →
-      valid_transition prov lbl tr
-.
-
-(*
- * Checks against the list element, can it be released via the current label?
- *)
-Inductive label_transition_valid_impl: prov_type → Policy.policy → list (trace_ty) → Prop :=
-  | LabelTransitionImplNil: ∀ prov lbl, label_transition_valid_impl prov lbl nil
-  | LabelTransitionImplCons: ∀ prov lbl tr hd tl,
-      tr = hd :: tl →
-      label_transition_valid_impl prov lbl tl →
-      (* hd: old trace (higher) *)
-      valid_transition prov lbl hd →
-      label_transition_valid_impl prov lbl tr
-.
-
-Inductive binary_ok: prov_type → Policy.policy → trace_ty → trace_ty → Prop :=
-  | BinaryOkAllEmpty: ∀ prov lbl trace1 trace2,
-    (* Basically we can do anything with non-policy guarded data. *)
-      trace1 = TrEmpty (∎) ∧ trace2 = TrEmpty (∎) →
-      binary_ok prov lbl trace1 trace2
-  | BinaryOkCannotDisclose: ∀ prov lbl trace1 trace2,
-      lbl = (∘ Policy.policy_top) →
-      binary_ok prov lbl trace1 trace2
-  | BinaryOkLhsEmpty: ∀ prov lbl trace1 trace2,
-      extract_policy trace1 = ∎ →
-      valid_transition prov lbl trace2 →
-      binary_ok prov lbl trace1 trace2
-  | BinaryOkRhsEmpty: ∀ prov lbl trace1 trace2,
-      extract_policy trace2 = ∎ →
-      valid_transition prov lbl trace1 →
-      binary_ok prov lbl trace1 trace2
-.
-
-Inductive label_transition_valid: trace_ty → Prop :=
-  | LabelTransitionTrEmpty: ∀ p, label_transition_valid (TrEmpty p)
-  | LabelTransitionTrLinear: ∀ tr prov lbl l,
-      tr = TrLinear prov lbl l →
-      label_transition_valid_impl prov lbl (l :: nil) →
-      label_transition_valid tr
-  | LabelTransitionTrBranch: ∀ tr lbl prov trace,
-      tr = TrBranch prov lbl trace →
-      Forall (λ x, label_transition_valid x) trace →
-      branch_ok lbl trace →
-      label_transition_valid tr
-  | LabelTransitionTrBinary: ∀ tr prov lbl trace1 trace2,
-    tr = TrBinary prov lbl trace1 trace2 →
-    binary_ok prov lbl trace1 trace2 →
-    label_transition_valid tr
-.
-
-(*
- * We iterate over the trace information and checks for each cell id if its
- * corresponding policy transition is indeed valid and enforced in the course of
- * the query execution trace.
- *
- * This somehow resembles the following Fixpoint function:
- *
- * Fixpoint trace_ok tr :=
- *  match tr with
- *  | nil => True
- *  | hd :: tl => label_transition_valid (snd hd) ∧ trace_ok tl
- *  end.
- *)
-Inductive trace_ok: trace → Prop :=
-  | TraceEmpty: trace_ok nil
-  | TraceCons: ∀ tr hd tl,
-      tr = hd :: tl →
-      label_transition_valid (snd hd) →
-      trace_ok tl →
-      trace_ok (hd :: tl)
-.
-
-(*
- * Checks if the trace faithfully "mirror"s the policy context.
- *)
-Definition trace_consistent (tr: ctx trace_ty) (Γ: ctx Policy.policy): Prop :=
-  match tr with
-  | nil => True
-  | (id, tr_ty) :: tl =>
-    match label_lookup Γ id with
-    | Some p => p ⪯ (extract_policy tr_ty)
-    | None => False
-    end
-  end.
-
-(* Definition trace_valid tr Γ := *)
-
-Lemma label_transition_valid_impl_merge_app: ∀ body1 body2 prov lbl,
-  label_transition_valid_impl prov lbl body1 ∧
-  label_transition_valid_impl prov lbl body2 →
-  label_transition_valid_impl prov lbl (body1 ++ body2).
-Proof.
-  induction body1; intros; simpl in *; intuition.
-  induction body2.
-  - rewrite app_nil_r. auto.
-  - econstructor; eauto.
-    + eapply IHbody1. split.
-      * inversion H0. subst. inversion H. subst. assumption.
-      * assumption.
-    + inversion H0. subst. inversion H. subst. assumption.
-Qed.
-
-Lemma trace_ok_app_cons_tail: ∀ a tr1 tr2,
-   trace_ok (tr1 ++ tr2) ∧ label_transition_valid (snd a) →
-   trace_ok (tr1 ++ a :: tr2).
-Proof.
-  induction tr1; intros; simpl in *; intuition; (econstructor; eauto); inversion H0.
-  - assumption.
-  - subst. apply IHtr1. econstructor; eauto.
-Qed.
-
-Lemma trace_ok_app_comm: ∀ tr1 tr2,
-  trace_ok (tr1 ++ tr2) →
-  trace_ok (tr2 ++ tr1).
-Proof.
-  induction tr1; intros; simpl in *.
-  - rewrite app_nil_r. assumption.
-  - inversion H. subst. apply IHtr1 in H4.
-    apply trace_ok_app_cons_tail. intuition.
-Qed.
-
-Lemma update_label_trace_ok_spec: ∀ tr id tr_new,
-  trace_ok tr ∧ label_transition_valid tr_new →
-  trace_ok (update_label tr id tr_new).
-Proof.
-  induction tr; intros; intuition.
-  simpl. destruct a. destruct (Nat.eqb id n) eqn: Hn.
-  - apply Nat.eqb_eq in Hn. subst.
-    inversion H0. subst.
-    econstructor; eauto. apply trace_ok_app_comm.
-    econstructor; eauto.
-  - inversion H0. subst. simpl. econstructor; eauto.
-Qed.
-
-Lemma label_lookup_no_effect: ∀ tr id item,
-  trace_ok tr →
-  label_lookup tr id = Some item →
-  label_transition_valid item.
-Proof.
-  induction tr.
-  - discriminate.
-  - intros. destruct a. simpl in H0. destruct (Nat.eqb id n) eqn: Hn.
-    + inversion H0; subst. inversion H; subst. auto.
-    + eapply IHtr; eauto. inversion H; subst. auto.
-Qed.
 
 Lemma database_get_contexts_trace_ok: ∀ db s r n β tr,
   database_get_contexts db n = Some (RelationWrapped s r, tr, β) →
@@ -449,14 +244,6 @@ Proof.
     apply inj_pair2_eq_dec in H1; try (apply basic_type_eq_dec). subst.
     assumption.
 Qed.
-
-Lemma do_eval_udf_ok: ∀ args_types ret op f β tr tp gb args policy trace res,
-  trace_ok tr →
-  do_eval_udf args_types ret op f (β, tr, tp, gb) args (Some (policy, trace, res)) →
-  Forall (λ x, label_transition_valid x) trace ∧ branch_ok policy trace.
-Proof.
-  
-Admitted.
 
 Lemma eval_udf_ok: ∀ arg_types ret op f args β β' tr tr' tp tp' gb gb' v,
   trace_ok tr →
@@ -1047,7 +834,7 @@ Proof.
         -- split.
           ++ econstructor; eauto.
           ++ split; intuition.
-      * destruct (bounded_list_dec _ (a0 :: s) g).
+      * destruct (Util.bounded_list_dec _ (a0 :: s) g).
         -- destruct (determine_schema_agg (a0 :: s) a g b) as [s_agg|] eqn: Hdet.
            ++ destruct (eval_aggregate_terminate (a0 :: s) s_agg g b a e β tr (t :: r)) as [res Hterm].
               destruct res as [ [ [ r' β' ] tr' ] |].
