theories/Base/Trace.v
@@ -1,0 +1,281 @@
+Require Import Arith.
+Require Import List.
+Require Import Unicode.Utf8.
+
+Require Import DataModel.
+Require Import Types.
+Require Import Util.
+
+Inductive prov_type: Set :=
+  | prov_trans_unary: un_op → prov_type
+  | prov_trans_binary: ∀ bt, bin_op → type_to_coq_type bt → prov_type
+  | prov_agg: agg_op → prov_type
+  (* Just re-use it; should be fine. *)
+  | prov_udf: trans_op → prov_type
+  | prov_noise: noise_op → prov_type
+  | prov_join: prov_type
+.
+
+Definition prov_type_eqb (τ1 τ2: prov_type): bool.
+  refine (match τ1, τ2 with
+  | prov_trans_unary op1, prov_trans_unary op2 => un_op_eqb op1 op2
+  | prov_trans_binary bt1 op1 v1, prov_trans_binary bt2 op2 v2 => andb (bin_op_eqb op1 op2) _
+  | prov_agg op1, prov_agg op2 => agg_op_eqb op1 op2
+  | prov_noise op1, prov_noise op2 => noise_op_eqb op1 op2
+  | prov_join, prov_join => true
+  | prov_udf op1, prov_udf op2 => trans_op_eqb op1 op2
+  | _, _ => false
+  end).
+  destruct (type_matches bt1 bt2) eqn: Heq.
+  - apply type_matches_eq in Heq. subst.
+    destruct bt2; simpl in *.
+    + destruct (Nat.eqb v1 v2).
+      * apply true.
+      * apply false.
+    + destruct (Bool.eqb v1 v2).
+      * apply true.
+      * apply false.
+    + destruct (String.eqb v1 v2).
+      * apply true.
+      * apply false.
+  - apply false.
+Defined.
+
+Inductive trace_ty: Type :=
+  (* ⊥ *)
+  | TrEmpty: Policy.policy → trace_ty
+  (* Linear trace: op → current policy → predecessors *)
+  | TrLinear: prov_type → Policy.policy → trace_ty → trace_ty
+  (* Branching trace. *)
+  | TrBranch: prov_type → Policy.policy → list trace_ty → trace_ty
+  (* Binary expressions *)
+  | TrBinary: prov_type → Policy.policy → trace_ty → trace_ty → trace_ty  
+.
+
+Definition extract_policy tr :=
+  match tr with
+  | TrEmpty p => p
+  | TrLinear _ p _ => p
+  | TrBranch _ p _ => p
+  | TrBinary _ p _ _ => p
+  end.
+
+(*
+ * A trace is a list of tuples recording how a given data cell is transitioned
+ * from one policy to another; it also bookkeeps the provenance information.
+ *)
+Definition trace := ctx trace_ty.
+
+(* σ ::= ⟨ Γ, β ⟩; the program state. *)
+Definition σ := (Policy.context * budget)%type.
+
+
+(*
+ * Checks whether a policy p1 can be downgraded to p2 using op.
+ *)
+Definition valid_prov (τ: prov_type) (p1 p2: Policy.policy): Prop :=
+  (*
+   * First of all we must ensure that the level of policies are lowered, which would
+   * otherwise make no sense at all.
+   *)
+  p2 ⪯ p1 ∧
+  (*
+   * Next we check if `p1` can be "lowered". This is ensured by `p1` ⪯ `∘ op`
+   *)
+    match τ with
+      (*
+      * Adding `p ⪯ ∘ op` should be enough for the condition as this is equivalent to
+      * `(first label p) ⊑ op`, the proof of which is trivial and intuitive.
+      *)
+      | prov_trans_unary op => p2 ⪯ (∘ (Policy.policy_transform ((UnaryTransOp op) :: nil)))
+      | prov_trans_binary bt op v => p2 ⪯ (∘ (Policy.policy_transform ((BinaryTransOp bt op v) :: nil)))
+      | prov_agg op => p2 ⪯ (∘ (Policy.policy_agg (op :: nil)))
+      | prov_noise op => p2 ⪯ (∘ (Policy.policy_noise op))
+      | _ => True
+    end
+.
+
+(*
+ * For a cell to be released (i.e., it can be shared freely), it must be the case that all policies are satisfied.
+ * Fortunately, we have `policy_clean`. This means that we can just check whether the policy is clean.
+ *)
+Definition can_release p: Prop := p = ∎.
+
+(* TODO: Define this. *)
+Definition budget_bounded (β: budget): Prop := True.
+
+Notation "p1 '=[' p ']=>' p2" := (valid_prov p p1 p2)
+  (at level 10, p at next level, p2 at next level).
+
+(* 
+ *                      ----< tr1
+ *                     /
+ * trace: join / agg --< lbl  -----< tr2
+ *                     \
+ *                      ----< ...
+ *)
+Inductive branch_ok: Policy.policy → list trace_ty → Prop :=
+  | BranchEmptyOk: ∀ lbl, branch_ok lbl nil
+  | BranchConsOk: ∀ lbl lbl1 tr hd tl,
+      tr = hd :: tl →
+      lbl1 = extract_policy hd →
+      lbl1 ⪯ lbl →
+      branch_ok lbl tl →
+      branch_ok lbl tr
+.
+
+(*
+ * Checks against for each element, can it be released via the current label?
+ *)
+Inductive valid_transition: prov_type → Policy.policy → trace_ty → Prop :=
+  (* tr: old (higher) *)
+  (* lbl: new (lower) *)
+  | ValidTransition: ∀ prov lbl lbl' tr,
+      lbl' = extract_policy tr →
+      lbl' =[ prov ]=> lbl →
+      valid_transition prov lbl tr
+.
+
+(*
+ * Checks against the list element, can it be released via the current label?
+ *)
+Inductive label_transition_valid_impl: prov_type → Policy.policy → list (trace_ty) → Prop :=
+  | LabelTransitionImplNil: ∀ prov lbl, label_transition_valid_impl prov lbl nil
+  | LabelTransitionImplCons: ∀ prov lbl tr hd tl,
+      tr = hd :: tl →
+      label_transition_valid_impl prov lbl tl →
+      (* hd: old trace (higher) *)
+      valid_transition prov lbl hd →
+      label_transition_valid_impl prov lbl tr
+.
+
+Inductive binary_ok: prov_type → Policy.policy → trace_ty → trace_ty → Prop :=
+  | BinaryOkAllEmpty: ∀ prov lbl trace1 trace2,
+    (* Basically we can do anything with non-policy guarded data. *)
+      trace1 = TrEmpty (∎) ∧ trace2 = TrEmpty (∎) →
+      binary_ok prov lbl trace1 trace2
+  | BinaryOkCannotDisclose: ∀ prov lbl trace1 trace2,
+      lbl = (∘ Policy.policy_top) →
+      binary_ok prov lbl trace1 trace2
+  | BinaryOkLhsEmpty: ∀ prov lbl trace1 trace2,
+      extract_policy trace1 = ∎ →
+      valid_transition prov lbl trace2 →
+      binary_ok prov lbl trace1 trace2
+  | BinaryOkRhsEmpty: ∀ prov lbl trace1 trace2,
+      extract_policy trace2 = ∎ →
+      valid_transition prov lbl trace1 →
+      binary_ok prov lbl trace1 trace2
+.
+
+Inductive label_transition_valid: trace_ty → Prop :=
+  | LabelTransitionTrEmpty: ∀ p, label_transition_valid (TrEmpty p)
+  | LabelTransitionTrLinear: ∀ tr prov lbl l,
+      tr = TrLinear prov lbl l →
+      label_transition_valid_impl prov lbl (l :: nil) →
+      label_transition_valid tr
+  | LabelTransitionTrBranch: ∀ tr lbl prov trace,
+      tr = TrBranch prov lbl trace →
+      Forall (λ x, label_transition_valid x) trace →
+      branch_ok lbl trace →
+      label_transition_valid tr
+  | LabelTransitionTrBinary: ∀ tr prov lbl trace1 trace2,
+    tr = TrBinary prov lbl trace1 trace2 →
+    binary_ok prov lbl trace1 trace2 →
+    label_transition_valid tr
+.
+
+(*
+ * We iterate over the trace information and checks for each cell id if its
+ * corresponding policy transition is indeed valid and enforced in the course of
+ * the query execution trace.
+ *
+ * This somehow resembles the following Fixpoint function:
+ *
+ * Fixpoint trace_ok tr :=
+ *  match tr with
+ *  | nil => True
+ *  | hd :: tl => label_transition_valid (snd hd) ∧ trace_ok tl
+ *  end.
+ *)
+Inductive trace_ok: trace → Prop :=
+  | TraceEmpty: trace_ok nil
+  | TraceCons: ∀ tr hd tl,
+      tr = hd :: tl →
+      label_transition_valid (snd hd) →
+      trace_ok tl →
+      trace_ok (hd :: tl)
+.
+
+(*
+ * Checks if the trace faithfully "mirror"s the policy context.
+ *)
+Definition trace_consistent (tr: ctx trace_ty) (Γ: ctx Policy.policy): Prop :=
+  match tr with
+  | nil => True
+  | (id, tr_ty) :: tl =>
+    match label_lookup Γ id with
+    | Some p => p ⪯ (extract_policy tr_ty)
+    | None => False
+    end
+  end.
+
+(* Definition trace_valid tr Γ := *)
+
+Lemma label_transition_valid_impl_merge_app: ∀ body1 body2 prov lbl,
+  label_transition_valid_impl prov lbl body1 ∧
+  label_transition_valid_impl prov lbl body2 →
+  label_transition_valid_impl prov lbl (body1 ++ body2).
+Proof.
+  induction body1; intros; simpl in *; intuition.
+  induction body2.
+  - rewrite app_nil_r. auto.
+  - econstructor; eauto.
+    + eapply IHbody1. split.
+      * inversion H0. subst. inversion H. subst. assumption.
+      * assumption.
+    + inversion H0. subst. inversion H. subst. assumption.
+Qed.
+
+Lemma trace_ok_app_cons_tail: ∀ a tr1 tr2,
+   trace_ok (tr1 ++ tr2) ∧ label_transition_valid (snd a) →
+   trace_ok (tr1 ++ a :: tr2).
+Proof.
+  induction tr1; intros; simpl in *; intuition; (econstructor; eauto); inversion H0.
+  - assumption.
+  - subst. apply IHtr1. econstructor; eauto.
+Qed.
+
+Lemma trace_ok_app_comm: ∀ tr1 tr2,
+  trace_ok (tr1 ++ tr2) →
+  trace_ok (tr2 ++ tr1).
+Proof.
+  induction tr1; intros; simpl in *.
+  - rewrite app_nil_r. assumption.
+  - inversion H. subst. apply IHtr1 in H4.
+    apply trace_ok_app_cons_tail. intuition.
+Qed.
+
+Lemma update_label_trace_ok_spec: ∀ tr id tr_new,
+  trace_ok tr ∧ label_transition_valid tr_new →
+  trace_ok (update_label tr id tr_new).
+Proof.
+  induction tr; intros; intuition.
+  simpl. destruct a. destruct (Nat.eqb id n) eqn: Hn.
+  - apply Nat.eqb_eq in Hn. subst.
+    inversion H0. subst.
+    econstructor; eauto. apply trace_ok_app_comm.
+    econstructor; eauto.
+  - inversion H0. subst. simpl. econstructor; eauto.
+Qed.
+
+Lemma label_lookup_no_effect: ∀ tr id item,
+  trace_ok tr →
+  label_lookup tr id = Some item →
+  label_transition_valid item.
+Proof.
+  induction tr.
+  - discriminate.
+  - intros. destruct a. simpl in H0. destruct (Nat.eqb id n) eqn: Hn.
+    + inversion H0; subst. inversion H; subst. auto.
+    + eapply IHtr; eauto. inversion H; subst. auto.
+Qed.
