theories/Experimental/Udf.v
@@ -1,0 +1,23 @@
+Require Import Eqdep_dec.
+Require Import List.
+Require Import Unicode.Utf8.
+
+Require Import Base.Trace.
+
+Require Import Operational.Expression.
+
+Lemma do_eval_udf_ok: ∀ trace args_types ret op f β tr tp gb args policy res,
+  trace_ok tr →
+  do_eval_udf args_types ret op f (β, tr, tp, gb) args (Some (policy, trace, res)) →
+  Forall (λ x, label_transition_valid x) trace ∧ branch_ok policy trace.
+Proof.
+  induction trace.
+  - intuition. constructor.
+  - intros. inversion H0. subst. inversion H5. subst. clear H5. (* Preparation *)
+    apply inj_pair2_eq_dec in H1, H1, H4.
+    + inversion H15. subst.
+      inversion H7. subst. apply inj_pair2_eq_dec in H6. subst. split.
+      * apply Forall_cons_iff. split.
+        -- inversion H21. subst.
+
+Admitted.
