README.md
@@ -6,8 +6,13 @@ This repository contains formalization for the dataframe data model and relation
 
 We provide a quick introduction on how this Coq codebase relates to the on-paper formalism.
 
-TODO: Make things tidier by organizing things into sub-folders.
-
+- `Base`: The formalism of the basic mathemtical objects like lattices, types, ordering systems, etc. to build Picachv's data model as well as operational semantics.
+- `Data`: The formalism of the data model (Policies in Section 4. and relational data model in Section 5.).
+- `Experimental`: Some experiemental features and/or proofs not yet fully completed (User-Defined Functions and Termination proofs.). For experimental features, we aim to extend Picachv's formal model with the following features in the near future:
+  - User-Defined Functions: We outlined the operational semantics for these but working on finalizing them.
+  - Termination Proofs: We want to show that Picachv always gives an output.
+  - Differential privacy budget control and monitoring.
+- `Operational`: The formalism of the $\sf RA^P$ operational semantics and security proofs (The evaluation rules shown in Section 5.).
 ## Note
 
 The codebase of Picachv's Coq formalism is still untidy and will be cleaned up as soon as possible. As for now, there might some naming issues and/or inconsistent terms between the Coq code and paper descriptions. We sincerely apologize for any inconvenince and will fix it.
